theories/zoo/diaframe/specs.v
@@ -157,6 +157,22 @@ Section zoo_G.
     iSteps.
   Qed.
 
+  #[global] Instance get_tag_diaspec l E :
+    DIASPEC hdr
+    {{
+      l ↦ₕ hdr
+    }}
+      GetTag #l @ E
+    {{
+      RET #(encode_tag hdr.(header_tag));
+      True
+    }}.
+  Proof.
+    iSteps.
+    wp_get_tag.
+    iSteps.
+  Qed.
+
   #[global] Instance get_size_diaspec l E :
     DIASPEC hdr
     {{
