theories/zoo/language/syntax.v
@@ -242,6 +242,7 @@ Inductive expr :=
   | Alloc (e1 e2 : expr)
   | Block mut tag (es : list expr)
   | Match (e0 : expr) x (e1 : expr) (brs : list (pattern * expr))
+  | GetTag (e : expr)
   | GetSize (e : expr)
   | Load (e1 e2 : expr)
   | Store (e1 e2 e3 : expr)
@@ -332,6 +333,9 @@ Section expr_ind.
     ∀ e1, P e1 →
     ∀ brs, Forall (λ br, P br.2) brs →
     P (Match e0 x e1 brs).
+  Variable HGetTag :
+    ∀ e, P e →
+    P (GetTag e).
   Variable HGetSize :
     ∀ e, P e →
     P (GetSize e).
@@ -431,6 +435,9 @@ Section expr_ind.
           x
           e1 (expr_ind e1)
           brs (Forall_true (λ br, P br.2) brs (λ br, expr_ind br.2))
+    | GetTag e =>
+        HGetTag
+          e (expr_ind e)
     | GetSize e =>
         HGetSize
           e (expr_ind e)
@@ -563,6 +570,9 @@ Section expr_val_ind.
     ∀ e1, Pexpr e1 →
     ∀ brs, Forall (λ br, Pexpr br.2) brs →
     Pexpr (Match e0 x e1 brs).
+  Variable HGetTag :
+    ∀ e, Pexpr e →
+    Pexpr (GetTag e).
   Variable HGetSize :
     ∀ e, Pexpr e →
     Pexpr (GetSize e).
@@ -674,6 +684,9 @@ Section expr_val_ind.
           x
           e1 (expr_val_ind e1)
           brs (Forall_true (λ br, Pexpr br.2) brs (λ br, expr_val_ind br.2))
+    | GetTag e =>
+        HGetTag
+          e (expr_val_ind e)
     | GetSize e =>
         HGetSize
           e (expr_val_ind e)
@@ -992,6 +1005,9 @@ Proof.
             (decide (x1 = x2))
             (decide (e11 = e21))
             (decide (brs1 = brs2))
+      | GetTag e1, GetTag e2 =>
+          cast_if
+            (decide (e1 = e2))
       | GetSize e1, GetSize e2 =>
           cast_if
             (decide (e1 = e2))
@@ -1223,28 +1239,30 @@ Proof.
     11.
   #[local] Notation code_branch :=
     12.
-  #[local] Notation code_GetSize :=
+  #[local] Notation code_GetTag :=
     13.
-  #[local] Notation code_Load :=
+  #[local] Notation code_GetSize :=
     14.
-  #[local] Notation code_Store :=
+  #[local] Notation code_Load :=
     15.
-  #[local] Notation code_Xchg :=
+  #[local] Notation code_Store :=
     16.
-  #[local] Notation code_CAS :=
+  #[local] Notation code_Xchg :=
     17.
-  #[local] Notation code_FAA :=
+  #[local] Notation code_CAS :=
     18.
-  #[local] Notation code_Fork :=
+  #[local] Notation code_FAA :=
     19.
-  #[local] Notation code_GetLocal :=
+  #[local] Notation code_Fork :=
     20.
-  #[local] Notation code_SetLocal :=
+  #[local] Notation code_GetLocal :=
     21.
-  #[local] Notation code_Proph :=
+  #[local] Notation code_SetLocal :=
     22.
-  #[local] Notation code_Resolve :=
+  #[local] Notation code_Proph :=
     23.
+  #[local] Notation code_Resolve :=
+    24.
   #[local] Notation code_ValRecs :=
     0.
   #[local] Notation code_recursive :=
@@ -1289,6 +1307,8 @@ Proof.
           GenNode code_Block $ GenLeaf (EncodeMutability mut) :: GenLeaf (EncodeNat tag) :: go_list es
       | Match e0 x e1 brs =>
           GenNode code_Match $ go e0 :: GenLeaf (EncodeBinder x) :: go e1 :: go_branches brs
+      | GetTag e =>
+          GenNode code_GetTag [go e]
       | GetSize e =>
           GenNode code_GetSize [go e]
       | Load e1 e2 =>
@@ -1374,6 +1394,8 @@ Proof.
           Block mut tag $ go_list es
       | GenNode code_Match (e0 :: GenLeaf (EncodeBinder x) :: e1 :: brs) =>
           Match (go e0) x (go e1) (go_branches brs)
+      | GenNode code_GetTag [e] =>
+          GetTag (go e)
       | GenNode code_GetSize [e] =>
           GetSize (go e)
       | GenNode code_Load [e1; e2] =>
