theories/zoo/program_logic/wp.v
@@ -182,6 +182,21 @@ Section zoo_G.
       iApply (bwp_match_ctx with "Hl H"); first done.
   Qed.
 
+  Lemma wp_get_tag l hdr tid E Φ :
+    ▷ l ↦ₕ hdr -∗
+    ▷ Φ #(encode_tag hdr.(header_tag)) -∗
+    WP GetTag #l ∷ tid @ E {{ Φ }}.
+  Proof.
+    iIntros ">Hheader HΦ".
+    iApply bwp_wp_weak. iIntros.
+    iApply bwp_lift_atomic_base_step_nofork; first done. iIntros "%nt %σ1 %κs Hinterp".
+    iApply fupd_mask_intro; first set_solver. iIntros "Hclose".
+    iDestruct (state_interp_has_header_valid with "Hinterp Hheader") as %Hheaders_lookup.
+    iSplit; first eauto with zoo. iIntros "%κ %κs' %e %σ2 %es -> %Hstep _ !>".
+    invert_base_step.
+    iSteps.
+  Qed.
+
   Lemma wp_get_size l hdr tid E Φ :
     ▷ l ↦ₕ hdr -∗
     ▷ Φ #hdr.(header_size) -∗
